some revisions

theories/Context.v
@@ -4,11 +4,80 @@ From LambdaST Require Import
   Eqb
   FV
   Sets
-  Terms
   Types.
 From Coq Require Import
   List
   String.
+
+Fixpoint lcontains {T} `{Eqb T} x li :=
+  match li with
+  | nil => false
+  | cons hd tl => (eqb hd x || lcontains x tl)%bool
+  end.
+
+Lemma lcontains_in : forall {T} `{Eqb T} x li,
+  Bool.reflect (List.In x li) (lcontains x li).
+Proof.
+  intros. generalize dependent H. generalize dependent x.
+  induction li; cbn in *; intros. { constructor. intros []. }
+  destruct (eqb_spec a x). { constructor. left. assumption. }
+  specialize (IHli x H). sinvert IHli; constructor. { right. assumption. }
+  intros [C | C]; tauto.
+Qed.
+Hint Resolve lcontains_in : core.
+
+Lemma lcontains_app : forall {T} a b `{Eqb T} x,
+  lcontains x (a ++ b) = (lcontains x a || lcontains x b)%bool.
+Proof.
+  induction a; cbn in *; intros. { reflexivity. }
+  destruct (eqb_spec a x); cbn. { reflexivity. } apply IHa.
+Qed.
+Hint Resolve lcontains_app : core.
+
+Fixpoint lminus {T} `{Eqb T} x li :=
+  match li with
+  | nil => nil
+  | cons hd tl => if eqb x hd then lminus x tl else cons hd (lminus x tl)
+  end.
+
+Lemma lminus_eq : forall {T} li `{Eqb T} x,
+  lcontains x (lminus x li) = false.
+Proof.
+  induction li; cbn in *; intros. { reflexivity. }
+  destruct (eqb_spec x a). { apply IHli. }
+  cbn. destruct (eqb_spec a x). { subst. tauto. }
+  rewrite IHli. reflexivity.
+Qed.
+
+Lemma lminus_neq : forall {T} li `{Eqb T} x y,
+  x <> y ->
+  lcontains x (lminus y li) = lcontains x li.
+Proof.
+  induction li; cbn in *; intros. { reflexivity. }
+  destruct (eqb_spec a x). {
+    subst. destruct (eqb_spec y x). { subst. tauto. } cbn. destruct (eqb_spec x x). { reflexivity. } tauto. }
+  destruct (eqb_spec y a). { subst. rewrite IHli; [| assumption]. reflexivity. }
+  cbn. destruct (eqb_spec a x). { subst. tauto. } rewrite IHli; [| assumption]. reflexivity.
+Qed.
+
+Fixpoint lsubset {T} `{Eqb T} small big :=
+  match small with
+  | nil => true
+  | cons hd tl => (lcontains hd big && lsubset tl big)%bool
+  end.
+
+Lemma lsubset_incl : forall {T} `{Eqb T} small big,
+  Bool.reflect (forall x, List.In x small -> List.In x big) (lsubset small big).
+Proof.
+  intros. generalize dependent H. generalize dependent big.
+  induction small; cbn in *; intros. { constructor. intros _ []. }
+  destruct (lcontains_in a big). 2: { constructor. intro C. apply n. apply C. left. reflexivity. }
+  specialize (IHsmall big H). sinvert IHsmall; constructor; intros.
+  - destruct H2; [subst | apply H1]; assumption.
+  - intro C. apply H1. intros. apply C. right. assumption.
+Qed.
+Hint Resolve lsubset_incl : core.
+
 
 Inductive context : Set :=
   | CtxEmpty
